src/tls/Negotiation.Version.fst
@@ -469,16 +469,14 @@ let isSentinelRandomValue client_pv server_pv server_random =
   (server_pv `leqPV` TLS_1p1 && TLS_1p2 `leqPV` client_pv && server_random = down @| abyte 0z)
 // TODO do we produce them? do we get downgrade resistance from them?
 
-module SH = Parsers.RealServerHello
-
 /// ServerHello sets the protocol version
 let chosen sh =
-  let pv0 = sh.SH.version in
+  let pv0 = HSM.sh_version sh in
   if TLS_1p3 `leqPV` pv0 then
     fatal Illegal_parameter "Server selected an illegal legacy protocol version"
   else
     let open Parsers.ServerHelloExtension in
-    match List.Tot.find SHE_supported_versions? sh.SH.extensions with
+    match List.Tot.find SHE_supported_versions? (HSM.sh_extensions sh) with
       | None -> correct pv0 // old style
       | Some (SHE_supported_versions pv1) ->
         if TLS_1p3 `leqPV` pv1 && pv0 <> TLS_1p2 then
@@ -498,7 +496,7 @@ let accept cfg sh (*pv ses sr*) =
   match chosen sh with
   | Error z -> Error z
   | Correct pv ->
-    if isSentinelRandomValue cfg.max_version pv sh.SH.random then
+    if isSentinelRandomValue cfg.max_version pv (HSM.sh_random sh) then
       fatal Illegal_parameter "Protocol-version downgrade attempt detected"
     else
     if not (supported cfg pv) then
